\documentclass[12pt, twoside]{article}
\usepackage[francais]{babel}
\usepackage[T1]{fontenc}
\usepackage[latin1]{inputenc}
\usepackage[left=7mm, right=7mm, top=7mm, bottom=7mm]{geometry}
\usepackage{float}
\usepackage{graphicx}
\usepackage{array}
\usepackage{multirow}
\usepackage{amsmath,amssymb,mathrsfs}
\usepackage{soul}
\usepackage{textcomp}
\usepackage{eurosym}
 \usepackage{variations}
\usepackage{tabvar}

\pagestyle{empty}

\begin{document}

\begin{flushleft}
NOM PRENOM: \ldots \ldots \ldots \ldots \ldots \ldots \ldots \ldots \ldots
 
\bigskip

\end{flushleft}

\begin{center}
{\fbox{$4^{e}3$ \qquad \qquad \textbf{\Large{Mini-test 3 (sujet 1)}}
\qquad \qquad 12/11/2013}}
\end{center}



\bigskip 


\ul{Exercice 1}: Calculer. 

\enskip

$A = -25 + 13 = \ldots \ldots \ldots $ \qquad \qquad \quad $B = 17 - 19 = \ldots
\ldots \ldots$ \qquad \qquad \quad 
$C = 30 - 24 = \ldots \ldots \ldots$

\enskip

\qquad \quad $D = - 6,2 - 2,4 = \ldots \ldots \ldots$ \qquad \qquad \qquad
$E = 24,1 + 3,8 = \ldots \ldots \ldots$


\bigskip

\bigskip


\ul{Exercice 2}: Donner l'écriture simplifiée (on n'effectuera pas les calculs). 

\enskip

$F = (-2) + (-6) = \ldots \ldots \ldots \ldots \ldots$ 


\enskip


$G = (+7,6) - (+3,2) = \ldots \ldots \ldots \ldots \ldots$


\enskip

$H = (-4,16) - (-8,9) = \ldots \ldots \ldots \ldots \ldots$


\enskip

$I = 14 + (-13) - (+17) + (-3,6) = \ldots \ldots \ldots \ldots \ldots$

\bigskip


\bigskip

\bigskip


\begin{flushleft}
NOM PRENOM: \ldots \ldots \ldots \ldots \ldots \ldots \ldots \ldots \ldots
 
\bigskip

\end{flushleft}

\begin{center}
{\fbox{$4^{e}3$ \qquad \qquad \textbf{\Large{Mini-test 3 (sujet 2)}}
\qquad \qquad 12/11/2013}}
\end{center}



\bigskip 


\ul{Exercice 1}: Calculer. 

\enskip

$A = 28-15 = \ldots \ldots \ldots $ \qquad \qquad \quad $B = 33-40 = \ldots
\ldots \ldots$ \qquad \qquad \quad 
$C = -56+12 = \ldots \ldots \ldots$

\enskip

\qquad \quad $D = - 3,4 - 4,1 = \ldots \ldots \ldots$ \qquad \qquad \qquad
$E = 17,5 + 4,3 = \ldots \ldots \ldots$


\bigskip

\bigskip



\ul{Exercice 2}: Donner l'écriture simplifiée (on n'effectuera pas les calculs). 

\enskip

$F = (+9,4) - (+7,2) = \ldots \ldots \ldots \ldots \ldots$ 


\enskip


$G = (-5,1) - (-4,2) = \ldots \ldots \ldots \ldots \ldots$


\enskip

$H = (-4) + (-10) = \ldots \ldots \ldots \ldots \ldots$


\enskip

$I = 16 + (-20) - (+15) + (-4,7) = \ldots \ldots \ldots \ldots \ldots$



\pagebreak




\begin{flushleft}
NOM PRENOM: \ldots \ldots \ldots \ldots \ldots \ldots \ldots \ldots \ldots
 
\bigskip

\end{flushleft}

\begin{center}
{\fbox{$4^{e}3$ \qquad \qquad \textbf{\Large{Mini-test 3 (sujet 1)}}
\qquad \qquad 12/11/2013}}
\end{center}



\bigskip 


\ul{Exercice 1}: Calculer. 

\enskip

$A = -25 + 13 = \ldots \ldots \ldots $ \qquad \qquad \qquad \quad $B = 17 - 19 =
\ldots \ldots \ldots$ \qquad \qquad \qquad \quad 
$C = 30 - 24 = \ldots \ldots \ldots$

\enskip

\qquad \qquad \quad $D = - 6,2 - 2,4 = \ldots \ldots \ldots$ \qquad \qquad
\qquad \qquad $E = (+26)+(-13) = \ldots \ldots \ldots$


\enskip

$F=(-46)+(-11)=\ldots \ldots \ldots \ldots$ \qquad \qquad \qquad 
$G=(-18)-(-14)=\ldots \ldots \ldots$


\bigskip

\bigskip


\ul{Exercice 2}: Donner l'écriture simplifiée (on n'effectuera pas les calculs). 

\enskip

$H = (-2) + (-6) = \ldots \ldots \ldots \ldots \ldots$ 


\enskip


$I = (+7,6) - (+3,2) = \ldots \ldots \ldots \ldots \ldots$


\enskip

$J = (-4,16) - (-8,9) = \ldots \ldots \ldots \ldots \ldots$



\bigskip


\bigskip

\bigskip


\begin{flushleft}
NOM PRENOM: \ldots \ldots \ldots \ldots \ldots \ldots \ldots \ldots \ldots
 
\bigskip

\end{flushleft}

\begin{center}
{\fbox{$4^{e}3$ \qquad \qquad \textbf{\Large{Mini-test 3 (sujet 2)}}
\qquad \qquad 12/11/2013}}
\end{center}



\bigskip 


\ul{Exercice 1}: Calculer. 

\enskip

$A = 28-15 = \ldots \ldots \ldots $ \qquad \qquad \quad \quad $B = 33-40 =
\ldots \ldots \ldots$ \qquad \qquad \quad \quad 
$C = -56+12 = \ldots \ldots \ldots$

\enskip

\qquad \quad \qquad $D = - 3,4 - 4,1 = \ldots \ldots \ldots$ \qquad \qquad
\qquad \qquad  \quad $E = (+14)+(-31) = \ldots \ldots \ldots$

\enskip


$F=(-25)+(-13)=\ldots \ldots \ldots$ \qquad \qquad \qquad  
$G=(-21)-(-8)=\ldots \ldots \ldots$
\bigskip

\bigskip



\ul{Exercice 2}: Donner l'écriture simplifiée (on n'effectuera pas les calculs). 

\enskip

$H = (+9,4) - (+7,2) = \ldots \ldots \ldots \ldots \ldots$ 


\enskip


$I = (-5,1) - (-4,2) = \ldots \ldots \ldots \ldots \ldots$


\enskip

$J = (-4) + (-10) = \ldots \ldots \ldots \ldots \ldots$


\end{document}
